extraction/src/ErgoTopUtil.ml
@@ -1,0 +1,24 @@
+(*
+ * Licensed under the Apache License, Version 2.0 (the "License");
+ * you may not use this file except in compliance with the License.
+ * You may obtain a copy of the License at
+ *
+ * http://www.apache.org/licenses/LICENSE-2.0
+ *
+ * Unless required by applicable law or agreed to in writing, software
+ * distributed under the License is distributed on an "AS IS" BASIS,
+ * WITHOUT WARRANTIES OR CONDITIONS OF ANY KIND, either express or implied.
+ * See the License for the specific language governing permissions and
+ * limitations under the License.
+ *)
+
+open ErgoComp.ErgoCompiler
+
+let my_init_repl_context input =
+  begin match brand_model_from_inputs input with
+  | Success bm -> init_repl_context bm input
+  | Failure e -> ErgoUtil.ergo_raise e
+  end
+let my_ergo_repl_eval_decl rctxt decl =
+  ergo_repl_eval_decl rctxt.ErgoComp.repl_context_brand_model rctxt decl
+    
