mechanization/Translation/ErgoTypetoErgoCType.v
@@ -19,10 +19,63 @@ Require Import List.
 
 Require Import ErgoSpec.Common.Utils.ENames.
 Require Import ErgoSpec.Common.Utils.EResult.
+Require Import ErgoSpec.Common.Utils.EProvenance.
 Require Import ErgoSpec.Common.Utils.EAstUtil.
 Require Import ErgoSpec.Common.Types.ErgoType.
 Require Import ErgoSpec.ErgoC.Lang.ErgoC.
 Require Import ErgoSpec.Backend.ErgoBackend.
+
+Section ErgoTypeExpansion.
+  Definition expand_hierarchy : Set := list string.
+  Definition expanded_type : Set := list (string * laergo_type).
+  Definition expand_ctxt : Set := list (string * (expand_hierarchy * expanded_type)).
+
+  (** Assumes decls sorted in topological order *)
+  Definition ergo_expand_extends
+             (ctxt:expand_ctxt)
+             (this:absolute_name)
+             (super:absolute_name)
+             (localtype:list (string * laergo_type)) : expand_ctxt :=
+    match lookup string_dec ctxt super with
+    | None => ctxt (** XXX Should be a system error *)
+    | Some (hierarchy, etype) =>
+      (this, (super::hierarchy,etype ++ localtype)) :: ctxt
+    end.
+
+  Definition ergo_decl_expand_extends (ctxt:expand_ctxt)
+             (this:absolute_name)
+             (decl_desc:laergo_type_declaration_desc) : expand_ctxt :=
+    match decl_desc with
+    | ErgoTypeEnum _ => ctxt
+    | ErgoTypeTransaction e _ => ctxt
+    | ErgoTypeConcept None rtl =>
+      (this, (nil, rtl)) :: ctxt
+    | ErgoTypeConcept (Some super) rtl =>
+      ergo_expand_extends ctxt this super rtl
+    | ErgoTypeEvent e _ => ctxt
+    | ErgoTypeAsset e _ => ctxt
+    | ErgoTypeParticipant e _ => ctxt
+    | ErgoTypeGlobal _ => ctxt
+    | ErgoTypeFunction _ => ctxt
+    | ErgoTypeContract _ _ _ => ctxt
+    end.
+
+  Fixpoint ergo_expand_extends_in_declarations (decls:list laergo_type_declaration) : expand_ctxt :=
+    List.fold_left
+      (fun ctxt decl =>
+         ergo_decl_expand_extends
+           ctxt
+           decl.(type_declaration_name)
+           decl.(type_declaration_type))
+      decls nil.
+
+  Definition ergo_hierarchy_from_expand (ctxt : expand_ctxt) :=
+    List.concat
+      (List.map (fun xyz =>
+                   List.map (fun x => (fst xyz, x)) (fst (snd xyz)))
+                ctxt).
+
+End ErgoTypeExpansion.
 
 Section ErgoTypetoErgoCType.
   Context {m:brand_relation}.
@@ -52,4 +105,148 @@ Section ErgoTypetoErgoCType.
     | ErgoTypeSum _ t1 t2 => teither (ergo_type_to_ergoc_type t1) (ergo_type_to_ergoc_type t2)
     end.
 
+  Definition ergo_ctype_decl_from_expand (ctxt : expand_ctxt) : tbrand_context_decls :=
+    List.map (fun xyz =>
+                (fst xyz,
+                 let rtl := snd (snd xyz) in
+                 trec
+                   open_kind
+                   (rec_sort (List.map (fun xy => (fst xy, ergo_type_to_ergoc_type (snd xy))) rtl))
+                   (rec_sort_sorted
+                      (List.map (fun xy => (fst xy, ergo_type_to_ergoc_type (snd xy))) rtl)
+                      (rec_sort (List.map (fun xy => (fst xy, ergo_type_to_ergoc_type (snd xy))) rtl))
+                      eq_refl))) ctxt.
+
 End ErgoTypetoErgoCType.
+
+Section TestModel.
+  Import ErgoCTypes.
+
+  Local Open Scope string.
+
+  (* For the CTO:
+     ============
+
+     concept Entity {}
+     concept Customer extends Entity { o Integer age o Integer cid o String name }
+     concept Purchase extends Entity { o Integer cid o String name o Integer pid o Integer quantity }
+   *)
+
+  Definition StoreHierarchy :=
+    ("org.accordproject.ergotop.Customer","org.accordproject.ergotop.Entity")::("org.accordproject.ergotop.Purchase","org.accordproject.ergotop.Entity")::nil.
+
+  Definition StoreBrandRelationMaybe : eresult tbrand_relation
+    := eresult_of_qresult dummy_provenance (mk_tbrand_relation StoreHierarchy).
+
+  Definition StoreBrandRelation : brand_relation :=
+    match StoreBrandRelationMaybe with
+    | Success _ _ s => s
+    | Failure _ _ e => tempty_brand_relation (* Not used *)
+    end.
+
+  (* Compute StoreBrandModelMaybe. *)
+  
+  Existing Instance StoreBrandRelation.
+
+  Program Definition EntityType : ergoc_type
+    := Rec Open nil _.
+
+  Program Definition CustomerType : ergoc_type
+    := Rec Open (("age", Nat)
+                 :: ("cid", Nat)
+                 :: ("name", String)
+                 :: nil) _.
+
+  Program Definition PurchaseType : ergoc_type
+    := Rec Open (("cid", Nat)
+                 :: ("name", String)
+                 :: ("pid", Nat)
+                 :: ("quantity", Nat)
+                 :: nil) _.
+
+  Definition StoreModelTypeDecls : tbrand_context_decls :=
+    (("org.accordproject.ergotop.Customer", CustomerType)
+     :: ("org.accordproject.ergotop.Entity", EntityType)
+     :: ("org.accordproject.ergotop.Purchase", PurchaseType)
+     :: nil).
+
+  Definition StoreBrandModelMaybe : eresult tbrand_model
+    := eresult_of_qresult dummy_provenance
+                          (mk_tbrand_model StoreModelTypeDecls).
+
+  (* Compute StoreBrandModelMaybe. *)
+  
+  Instance StoreBrandModel : brand_model :=
+    match StoreBrandModelMaybe with
+    | Success _ _ s => s
+    | Failure _ _ e => tempty_brand_model (* Not used *)
+    end.
+
+End TestModel.
+
+Section Translate.
+  Local Open Scope string.
+  Import ErgoCTypes.
+
+  Definition EntityDecl : laergo_type_declaration :=
+    mkErgoTypeDeclaration dummy_provenance "org.accordproject.ergotop.Entity"
+                          (ErgoTypeConcept None nil).
+  Definition CustomerDecl : laergo_type_declaration :=
+    mkErgoTypeDeclaration dummy_provenance "org.accordproject.ergotop.Customer"
+                          (ErgoTypeConcept (Some "org.accordproject.ergotop.Entity")
+                                           (("age",ErgoTypeInteger dummy_provenance)
+                                              ::("cid",ErgoTypeInteger dummy_provenance)
+                                              ::("name",ErgoTypeString dummy_provenance)
+                                              ::nil)).
+  Definition GoldCustomerDecl : laergo_type_declaration :=
+    mkErgoTypeDeclaration dummy_provenance "org.accordproject.ergotop.GoldCustomer"
+                          (ErgoTypeConcept (Some "org.accordproject.ergotop.Customer")
+                                           (("status",ErgoTypeString dummy_provenance)
+                                              ::nil)).
+  Definition PurchaseDecl : laergo_type_declaration :=
+    mkErgoTypeDeclaration dummy_provenance "org.accordproject.ergotop.Purchase"
+                          (ErgoTypeConcept (Some "org.accordproject.ergotop.Entity")
+                                           (("cid",ErgoTypeInteger dummy_provenance)
+                                              :: ("name",ErgoTypeString dummy_provenance)
+                                              :: ("pid",ErgoTypeInteger dummy_provenance)
+                                              :: ("quantity",ErgoTypeInteger dummy_provenance)
+                                              ::nil)).
+  Definition BearDecl : laergo_type_declaration :=
+    mkErgoTypeDeclaration dummy_provenance "org.accordproject.ergotop.Bear"
+                          (ErgoTypeConcept (Some "org.accordproject.ergotop.Entity")
+                                           (("name",ErgoTypeString dummy_provenance)
+                                              :: ("age",ErgoTypeInteger dummy_provenance)
+                                              ::nil)).
+  Definition StoreDecls : list laergo_type_declaration :=
+    EntityDecl :: CustomerDecl :: PurchaseDecl :: (* GoldCustomerDecl :: *) BearDecl :: nil. 
+  
+  (* Compute (hierarchy StoreDecls). *)
+  
+  Definition brand_relation_maybe hierarchy : eresult tbrand_relation
+    := eresult_of_qresult dummy_provenance (mk_tbrand_relation hierarchy).
+
+  (* Compute (brand_relation_maybe StoreDecls). *)
+
+  Definition mk_model_type_decls {br:brand_relation} (ctxt : expand_ctxt) : tbrand_context_decls :=
+    @ergo_ctype_decl_from_expand br ctxt.
+
+  Definition brand_model_of_declarations (decls:list laergo_type_declaration)
+    : eresult ErgoCTypes.tbrand_model :=
+    let ctxt := ergo_expand_extends_in_declarations decls in
+    let hierarchy := ergo_hierarchy_from_expand ctxt in
+    eolift (fun br =>
+              eresult_of_qresult dummy_provenance
+                                 (mk_tbrand_model (@mk_model_type_decls br ctxt)))
+           (brand_relation_maybe hierarchy).
+  
+  Definition force_brand_model_of_declarations (decls:list laergo_type_declaration)
+    : ErgoCTypes.tbrand_model :=
+    match brand_model_of_declarations decls with
+    | Success _ _ s => s
+    | Failure _ _ e => tempty_brand_model (* Not used *)
+    end.
+
+  (* Compute brand_model_of_declarations StoreDecls. *)
+
+End Translate.
+
